new_example/event_proof.v
@@ -15,70 +15,103 @@ Module Event_Proof.
       Program Instance : IsPkgInit main :=
         ltac2:(build_pkg_init ()).
 
-    Definition has_encoding (encoded:list u8) (args:main.Event.t) : Prop :=
-      ∃ start_enc end_enc,
-        encoded = (u32_le args.(main.Event.id')) ++
-                    (u64_le $ length $ args.(main.Event.name')) ++
-                    args.(main.Event.name') ++
-                    start_enc ++ end_enc
-        /\ length args.(main.Event.name') < 2^64
-        /\ TimeStamp_Proof.has_encoding start_enc args.(main.Event.startTime')
-        /\ TimeStamp_Proof.has_encoding end_enc args.(main.Event.endTime').
+    Record C :=
+      mkC {
+          id: u32;
+          name: go_string;
+          startTime: TimeStamp_Proof.C;
+          endTime: TimeStamp_Proof.C;
+      }.
 
-    Lemma wp_Encode (args__c:main.Event.t) (pre_sl:slice.t) (prefix:list u8) (dq:dfrac):
+    (* Definition has_encoding (encoded:list u8) (args:main.Event.t) : Prop := *)
+    (*   ∃ start_enc end_enc, *)
+    (*     encoded = (u32_le args.(main.Event.id')) ++ *)
+    (*                 (u64_le $ length $ args.(main.Event.name')) ++ *)
+    (*                 args.(main.Event.name') ++ *)
+    (*                 start_enc ++ end_enc *)
+    (*     /\ length args.(main.Event.name') < 2^64 *)
+    (*     /\ TimeStamp_Proof.has_encoding start_enc args.(main.Event.startTime') *)
+    (*     /\ TimeStamp_Proof.has_encoding end_enc args.(main.Event.endTime'). *)
+
+    Definition has_encoding' (encoded:list u8) (args:C) : Prop :=
+      ∃ start_enc end_enc,
+        encoded = (u32_le args.(id)) ++
+                    (u64_le $ length $ args.(name)) ++
+                    args.(name) ++
+                           start_enc ++ end_enc
+        /\ length args.(name) < 2^64
+        /\ TimeStamp_Proof.has_encoding' start_enc args.(startTime)
+        /\ TimeStamp_Proof.has_encoding' end_enc args.(endTime).
+
+    Definition own (v:main.Event.t) (c:C) (dq:dfrac) : iProp Σ :=
+      ⌜ v.(main.Event.id') = c.(id) ⌝ ∗
+      ⌜ v.(main.Event.name') = c.(name) ⌝ ∗
+      TimeStamp_Proof.own v.(main.Event.startTime') c.(startTime) dq ∗
+      TimeStamp_Proof.own v.(main.Event.endTime') c.(endTime) dq.
+
+    Lemma wp_Encode (args__t:main.Event.t) (args__c:C) (pre_sl:slice.t) (prefix:list u8) (dq:dfrac):
       {{{
             is_pkg_init main ∗
+            own args__t args__c dq ∗
             own_slice pre_sl (DfracOwn 1) prefix ∗
             own_slice_cap w8 pre_sl
       }}}
-        main @ "MarshalEvent" #pre_sl #args__c
+        main @ "MarshalEvent" #pre_sl #args__t
       {{{
             enc enc_sl, RET #enc_sl;
-            ⌜ has_encoding enc args__c ⌝ ∗
+            ⌜ has_encoding' enc args__c ⌝ ∗
             own_slice enc_sl (DfracOwn 1) (prefix ++ enc) ∗
-            own_slice_cap w8 enc_sl
+            own_slice_cap w8 enc_sl ∗
+            own args__t args__c dq
       }}}.
 
     Proof.
-      wp_start as "[Hsl Hcap]". wp_auto.
+      wp_start as "(Hown & Hsl & Hcap)". wp_auto.
+      iDestruct "Hown" as "(%Hid & %Hname & HstartTime & HendTime)".
 
       wp_apply (wp_WriteInt32 with "[$Hsl $Hcap]").
       iIntros (?) "[Hsl Hcap]". wp_auto.
 
       wp_apply wp_AssumeNoStringOverflow.
-      iIntros "%HnameLen". wp_auto.
+      iIntros "%HnameLen". rewrite Hname in HnameLen. wp_auto.
       wp_apply wp_StringToBytes.
       iIntros (?) "Hsl'". wp_auto.
 
       wp_apply (wp_WriteLenPrefixedBytes with "[$Hsl $Hsl' $Hcap]").
-      iIntros (?) "(Hs & Hcap & Hsl)". wp_auto.
+      iIntros (?) "(Hsl & Hcap & Hname)". wp_auto.
 
-      wp_apply (TimeStamp_Proof.wp_Encode with "[$Hs $Hcap]"); first trivial.
-      iIntros (??) "(%HstartTime & Hs & Hcap)". wp_auto.
+      wp_apply (TimeStamp_Proof.wp_Encode with "[$Hsl $Hcap $HstartTime]").
+      iIntros (??) "(%HstartTime & Hs & Hcap & HstartTime)". wp_auto.
 
-      wp_apply (TimeStamp_Proof.wp_Encode with "[$Hs $Hcap]"); first trivial.
-      iIntros (??) "(%HendTime & Hs & Hcap)". wp_auto.
+      wp_apply (TimeStamp_Proof.wp_Encode with "[$Hs $Hcap $HendTime]").
+      iIntros (??) "(%HendTime & Hs & Hcap & HendTime)". wp_auto.
 
       iApply "HΦ". rewrite -?app_assoc. iFrame.
-      iPureIntro. unfold has_encoding. exists enc, enc0.
+      iSplit.
+      {
+      iPureIntro. unfold has_encoding'. exists enc, enc0.
+      rewrite Hid. rewrite Hname.
       split; first reflexivity. done.
+      }
+      done.
     Qed.
 
-    Lemma wp_Decode (enc: list u8) (enc_sl: slice.t) (args__c:main.Event.t) (suffix: list u8) (dq: dfrac):
+    Lemma wp_Decode (enc: list u8) (enc_sl: slice.t) (args__c:C) (suffix: list u8) (dq: dfrac):
       {{{
             is_pkg_init main ∗
             own_slice enc_sl dq (enc ++ suffix) ∗
-            ⌜ has_encoding enc args__c ⌝
+            ⌜ has_encoding' enc args__c ⌝
       }}}
         main @ "UnmarshalEvent" #enc_sl
       {{{
-            suff_sl, RET (#args__c, #suff_sl);
-            own_slice suff_sl dq suffix
+            args__t suff_sl, RET (#args__t, #suff_sl);
+            own_slice suff_sl dq suffix ∗
+            own args__t args__c (DfracOwn 1)
       }}}.
 
     Proof.
       wp_start as "[Hsl %Henc]". wp_auto.
-      unfold has_encoding in Henc.
+      unfold has_encoding' in Henc.
       destruct Henc as (start_enc & end_enc & Henc & Hnlen & Henc_st & Henc_et).
       rewrite Henc. rewrite -?app_assoc.
 
@@ -88,22 +121,16 @@ Module Event_Proof.
       wp_apply (wp_ReadLenPrefixedBytes with "[$Hsl]"); first word.
       iIntros (??) "[Hn Hsl]". wp_auto.
 
-      wp_apply (TimeStamp_Proof.wp_Decode with "[$Hsl]"); first trivial.
-      iIntros (?) "Hsl". wp_auto.
+      wp_apply (TimeStamp_Proof.wp_Decode with "[$Hsl]"); first done.
+      iIntros (??) "[HstartTime Hsl]". wp_auto.
 
-      wp_apply (TimeStamp_Proof.wp_Decode with "[$Hsl]"); first trivial.
-      iIntros (?) "Hsl". wp_auto.
+      wp_apply (TimeStamp_Proof.wp_Decode with "[$Hsl]"); first done.
+      iIntros (??) "[HendTime Hsl]". wp_auto.
 
       wp_apply (wp_StringFromBytes with "[$Hn]").
       iIntros "Hn". wp_auto.
 
-      replace {|
-          main.Event.id' := args__c.(main.Event.id');
-          main.Event.name' := args__c.(main.Event.name');
-          main.Event.startTime' := args__c.(main.Event.startTime');
-          main.Event.endTime' := args__c.(main.Event.endTime')
-        |} with args__c; last (destruct args__c; reflexivity).
-      iApply "HΦ". iFrame.
+      iApply "HΦ". iFrame. done.
     Qed.
   End Event_Proof.
 End Event_Proof.
