new_example/timestamp_proof.v
@@ -1,4 +1,3 @@
-(* From Perennial.program_proof Require Import grove_prelude. *)
 From New.proof Require Import proof_prelude.
 From Grackle.new_ex Require Import goose.github_com.mjschwenne.grackle.new_example.
 From Grackle.new_ex Require Import pg.github_com.mjschwenne.grackle.new_example.
@@ -14,26 +13,45 @@ Module TimeStamp_Proof.
     Program Instance : IsPkgInit main :=
         ltac2:(build_pkg_init ()).
 
-    Definition has_encoding (encoded:list u8) (args:main.TimeStamp.t) : Prop :=
-      encoded = (u32_le args.(main.TimeStamp.hour')) ++ (u32_le args.(main.TimeStamp.minute'))
-                  ++ (u32_le args.(main.TimeStamp.second')).
+    Record C :=
+      mkC {
+          hour: u32;
+          minute: u32;
+          second: u32;
+      }.
 
-    Lemma wp_Encode (args__c : main.TimeStamp.t) (pre_sl : slice.t) (prefix : list u8) (dq : dfrac):
+    (* Definition has_encoding (encoded:list u8) (args:main.TimeStamp.t) : Prop := *)
+    (*   encoded = (u32_le args.(main.TimeStamp.hour')) ++ (u32_le args.(main.TimeStamp.minute')) *)
+    (*               ++ (u32_le args.(main.TimeStamp.second')). *)
+
+    Definition has_encoding' (encoded:list u8) (args:C) : Prop :=
+      encoded = (u32_le args.(hour)) ++ (u32_le args.(minute))
+                  ++ (u32_le args.(second)).
+
+    Definition own (v:main.TimeStamp.t) (c:C) (dq:dfrac) : iProp Σ :=
+      ⌜ v.(main.TimeStamp.hour') = c.(hour) ⌝ ∗
+      ⌜ v.(main.TimeStamp.minute') = c.(minute) ⌝ ∗
+      ⌜ v.(main.TimeStamp.second') = c.(second) ⌝. 
+
+    Lemma wp_Encode (args__t : main.TimeStamp.t) (args__c:C) (pre_sl : slice.t) (prefix : list u8) (dq : dfrac):
       {{{
             is_pkg_init main ∗
+            own args__t args__c dq ∗
             own_slice pre_sl (DfracOwn 1) prefix ∗
             own_slice_cap w8 pre_sl
       }}}
-        main @ "MarshalTimeStamp" #pre_sl #args__c
+        main @ "MarshalTimeStamp" #pre_sl #args__t
       {{{
             enc enc_sl, RET #enc_sl;
-            ⌜ has_encoding enc args__c ⌝ ∗
+            ⌜ has_encoding' enc args__c ⌝ ∗
             own_slice enc_sl (DfracOwn 1) (prefix ++ enc) ∗
-            own_slice_cap w8 enc_sl
+            own_slice_cap w8 enc_sl ∗
+            own args__t args__c dq
       }}}.
 
     Proof. 
-        wp_start as "[Hsl Hcap]". wp_auto.
+        wp_start as "(Hown & Hsl & Hcap)". wp_auto.
+        iDestruct "Hown" as "(%Hhour & %Hminute & %Hsecond)".
 
         wp_apply (wp_WriteInt32 with "[$Hsl $Hcap]").
         iIntros (?) "[Hsl Hcap]". wp_auto.
@@ -44,24 +62,28 @@ Module TimeStamp_Proof.
         wp_apply (wp_WriteInt32 with "[$Hsl $Hcap]").
         iIntros (?) "[Hsl Hcap]". wp_auto.
 
-        iApply "HΦ". rewrite -?app_assoc. iFrame. done.
+        iApply "HΦ". rewrite -?app_assoc. iFrame.
+        iPureIntro. unfold has_encoding'.
+        rewrite Hhour. rewrite Hminute. rewrite Hsecond.
+        done.
     Qed.
 
-    Lemma wp_Decode (enc: list u8) (enc_sl: slice.t) (args__c: main.TimeStamp.t) (suffix: list u8) (dq: dfrac):
+    Lemma wp_Decode (enc: list u8) (enc_sl: slice.t) (args__c:C) (suffix: list u8) (dq: dfrac):
       {{{
             is_pkg_init main ∗
             own_slice enc_sl dq (enc ++ suffix) ∗
-            ⌜ has_encoding enc args__c ⌝
+            ⌜ has_encoding' enc args__c ⌝
       }}}
         main @ "UnmarshalTimeStamp" #enc_sl
       {{{
-            suff_sl, RET (#args__c, #suff_sl);
+            args__t suff_sl, RET (#args__t, #suff_sl);
+            own args__t args__c dq ∗
             own_slice suff_sl dq suffix
       }}}.
         
     Proof.
       wp_start as "[Hsl %Henc]". wp_auto.
-      unfold has_encoding in Henc. rewrite Henc. rewrite -?app_assoc.
+      unfold has_encoding' in Henc. rewrite Henc. rewrite -?app_assoc.
 
       wp_apply (wp_ReadInt32 with "[$Hsl]").
       iIntros (?) "Hsl". wp_auto.
@@ -72,12 +94,12 @@ Module TimeStamp_Proof.
       wp_apply (wp_ReadInt32 with "[$Hsl]").
       iIntros (?) "Hsl". wp_auto.
 
-      replace {|
-       main.TimeStamp.hour' := args__c.(main.TimeStamp.hour');
-       main.TimeStamp.minute' := args__c.(main.TimeStamp.minute');
-       main.TimeStamp.second' := args__c.(main.TimeStamp.second')
-        |} with args__c; last (destruct args__c; reflexivity).
-      iApply "HΦ". iFrame.
+      (* replace {| *)
+      (*  main.TimeStamp.hour' := args__c.(hour); *)
+      (*  main.TimeStamp.minute' := args__c.(minute); *)
+      (*  main.TimeStamp.second' := args__c.(second) *)
+      (*   |} with args__t; last (destruct args__t; reflexivity). *)
+      iApply "HΦ". iFrame. done.
     Qed.
   End TimeStamp_Proof.
 End TimeStamp_Proof.
